Get examples/lambda/examples to build once more

examples/lambda/examples/holScript.sml
@@ -6,16 +6,15 @@ open basic_swapTheory nomsetTheory NEWLib
 
 val _ = new_theory "hol"
 
-fun Store_thm (n,t,tac) = store_thm(n,t,tac) before export_rewrites [n]
-
 (* a theory of higher order logic terms, as modelled in systems such as
    HOL4, Isabelle/HOL and HOL Light *)
 
 (* HOL types *)
 
-val _ = Hol_datatype `hol_type = tyvar of string
-                               | tyop of string => hol_type list
-`
+Datatype:
+  hol_type = tyvar string
+           | tyop string (hol_type list)
+End
 
 
 (*
@@ -26,18 +25,20 @@ it has to be
 
 *)
 
-val _ = Hol_datatype`raw_holterm = rhvar of string # hol_type
-                                 | rhconst of string # hol_type
-                                 | rhapp of raw_holterm => raw_holterm
-                                 | rhabs of string # hol_type => raw_holterm
-`
+
+Datatype:
+  raw_holterm = rhvar (string # hol_type)
+              | rhconst (string # hol_type)
+              | rhapp raw_holterm raw_holterm
+              | rhabs (string # hol_type) raw_holterm
+End
 
 (* but what is the appropriate notion of permutation on this type?
 
    It seems clear that it has to be the permutation of atoms that consist of
    names coupled with types *)
 
-val rawpm_def = Define`
+Definition rawpm_def[simp]:
   (rawpm ty pi (rhvar nty) = if ty = SND nty then
                                rhvar (lswapstr pi (FST nty), SND nty)
                              else rhvar nty) /\
@@ -47,125 +48,110 @@ val rawpm_def = Define`
      rhabs (if ty = SND nty then (lswapstr pi (FST nty), SND nty)
             else nty)
            (rawpm ty pi t))
-`;
-val _ = export_rewrites ["rawpm_def"]
+End
 
-val rawpm_is_perm = Store_thm(
-  "rawpm_is_perm",
-  ``!ty. is_perm (rawpm ty)``,
-  SRW_TAC [][is_perm_def] THENL [
-    Induct_on `x` THEN SRW_TAC [][],
-    Induct_on `x` THEN SRW_TAC [][lswapstr_APPEND] THEN
-    FULL_SIMP_TAC (srw_ss()) [],
-    FULL_SIMP_TAC (srw_ss()) [permeq_def, FUN_EQ_THM] THEN
-    Induct THEN SRW_TAC [][]
-  ]);
+Theorem rawpm_is_perm:
+  !ty. is_pmact (rawpm ty)
+Proof
+  SRW_TAC [][is_pmact_def]
+  >- (Induct_on `x` THEN SRW_TAC [][])
+  >- (Induct_on `x` >> rw[pmact_decompose] >> gvs[]) >>
+  simp[FUN_EQ_THM] >> Induct >> rw[] >>
+  metis_tac[pmact_permeq]
+QED
 
-val rawpms_differing_types_commute = store_thm(
-  "rawpms_differing_types_commute",
-  ``~(ty1 = ty2) ==>
-    (rawpm ty1 pi1 (rawpm ty2 pi2 t) =
-     rawpm ty2 pi2 (rawpm ty1 pi1 t))``,
-  Induct_on `t` THEN SRW_TAC [][] THEN METIS_TAC [])
+Overload rhpmact = “λty. mk_pmact (rawpm ty)”
+Overload rhpm = “λty. pmact (rhpmact ty)”
 
-val rawpm_nil = Store_thm(
-  "rawpm_nil",
-  ``rawpm ty [] t = t``,
-  METIS_TAC [is_perm_nil, rawpm_is_perm]);
+Theorem rawpm_rhpm:
+  rawpm ty = rhpm ty
+Proof
+  simp[GSYM pmact_bijections, rawpm_is_perm]
+QED
 
-val rawpm_APPEND = store_thm(
-  "rawpm_APPEND",
-  ``rawpm ty p1 (rawpm ty p2 t) = rawpm ty (p1 ++ p2) t``,
-  METIS_TAC [rawpm_is_perm, is_perm_decompose]);
+Theorem rhpm_thm[simp] = ONCE_REWRITE_RULE [rawpm_rhpm] rawpm_def
 
-val rawpm_inverse = Store_thm(
-  "rawpm_inverse",
-  ``(rawpm ty pi (rawpm ty (REVERSE pi) t) = t) /\
-    (rawpm ty (REVERSE pi) (rawpm ty pi t) = t)``,
-  METIS_TAC [rawpm_is_perm, is_perm_inverse]);
+Theorem rawpms_differing_types_commute:
+  ty1 ≠ ty2 ==>
+  rhpm ty1 pi1 (rhpm ty2 pi2 t) = rhpm ty2 pi2 (rhpm ty1 pi1 t)
+Proof
+  Induct_on `t` THEN SRW_TAC [][] THEN METIS_TAC []
+QED
 
-val rawpm_sing_inv = Store_thm(
-  "rawpm_sing_inv",
-  ``(rawpm ty [h] (rawpm ty [h] x) = x)``,
-  METIS_TAC [rawpm_is_perm, is_perm_sing_inv]);
-
-val rawpm_sing_to_back = store_thm(
-  "rawpm_sing_to_back",
-  ``rawpm ty [(lswapstr pi a, lswapstr pi b)] (rawpm ty pi t) =
-    rawpm ty pi (rawpm ty [(a,b)] t)``,
-  METIS_TAC [rawpm_is_perm, is_perm_sing_to_back]);
-
-val allvars_def = Define`
+Definition allvars_def[simp]:
   (allvars ty (rhvar nty) = if ty = SND nty then {FST nty} else {}) /\
   (allvars ty (rhconst nty) = {}) /\
   (allvars ty (rhapp t1 t2) = allvars ty t1 UNION allvars ty t2) /\
   (allvars ty (rhabs nty t) = (if ty = SND nty then {FST nty} else {}) UNION
                               allvars ty t)
-`;
-val _ = export_rewrites ["allvars_def"]
+End
 
-val IN_allvars_rawpm = Store_thm(
-  "IN_allvars_rawpm",
-  ``x IN allvars ty (rawpm ty pi t) =
-    lswapstr (REVERSE pi) x IN allvars ty t``,
-  Induct_on `t` THEN SRW_TAC [][lswapstr_eql] THEN
-  FULL_SIMP_TAC (srw_ss()) []);
+Theorem IN_allvars_rawpm[simp]:
+  x IN allvars ty (rhpm ty pi t) <=>
+  lswapstr (REVERSE pi) x IN allvars ty t
+Proof
+  Induct_on `t` >> simp[] >> rw[] >> SRW_TAC [][pmact_eql] >> gs[]
+QED
 
-val allvars_rawpm_diff = Store_thm(
-  "allvars_rawpm_diff",
-  ``~(ty1 = ty2) ==> (allvars ty1 (rawpm ty2 pi t) = allvars ty1 t)``,
-  Induct_on `t` THEN SRW_TAC [][] THEN METIS_TAC []);
+Theorem allvars_rawpm_diff[simp]:
+  ty1 ≠ ty2 ==> allvars ty1 (rhpm ty2 pi t) = allvars ty1 t
+Proof
+  Induct_on `t` THEN SRW_TAC [][] THEN METIS_TAC []
+QED
 
-val FINITE_allvars = Store_thm(
-  "FINITE_allvars",
-  ``FINITE (allvars ty t)``,
-  Induct_on `t` THEN SRW_TAC [][]);
+Theorem FINITE_allvars[simp]:
+  FINITE (allvars ty t)
+Proof
+  Induct_on `t` THEN SRW_TAC [][]
+QED
 
-val allvars_fresh = store_thm(
-  "allvars_fresh",
-  ``~(u IN allvars ty t) /\ ~(v IN allvars ty t) ==>
-    (rawpm ty [(u,v)] t = t)``,
-  Induct_on `t` THEN SRW_TAC [][]);
+Theorem allvars_fresh:
+  u ∉ allvars ty t ∧ v ∉ allvars ty t ⇒ rhpm ty [(u,v)] t = t
+Proof
+  Induct_on `t` THEN SRW_TAC [][]
+QED
 
-val (aeq_rules, aeq_ind, aeq_cases) = Hol_reln`
+Inductive aeq:
+[~var:]
   (!v. aeq (rhvar v) (rhvar v)) /\
+[~const:]
   (!v. aeq (rhconst v) (rhconst v)) /\
+[~app:]
   (!t1 t2 u1 u2. aeq t1 u1 /\ aeq t2 u2 ==>
                  aeq (rhapp t1 t2) (rhapp u1 u2)) /\
-  (!v1 v2 u t z.
+[~lam:]
+  (!v1 v2 u t z ty.
       ~(z IN allvars ty t) /\ ~(z IN allvars ty u) /\ ~(z = v1) /\
-      ~(z = v2) /\ aeq (rawpm ty [(z,v1)] t) (rawpm ty [(z,v2)] u) ==>
+      ~(z = v2) /\ aeq (rhpm ty [(z,v1)] t) (rhpm ty [(z,v2)] u) ==>
       aeq (rhabs (v1,ty) t) (rhabs (v2,ty) u))
-`;
+End
 
-val aeq_rawpm = store_thm(
-  "aeq_rawpm",
-  ``!t u. aeq t u ==> !pi ty. aeq (rawpm ty pi t) (rawpm ty pi u)``,
+Theorem aeq_rawpm:
+  !t u. aeq t u ==> !pi ty. aeq (rhpm ty pi t) (rhpm ty pi u)
+Proof
   HO_MATCH_MP_TAC aeq_ind THEN SRW_TAC [][aeq_rules] THEN
-  Cases_on `ty = ty'` THENL [
-    SRW_TAC [][] THEN
-    MATCH_MP_TAC (last (CONJUNCTS aeq_rules)) THEN
-    Q.EXISTS_TAC `lswapstr pi z` THEN SRW_TAC [][] THEN
-    SRW_TAC [][is_perm_sing_to_back, rawpm_is_perm],
-    SRW_TAC [][] THEN
-    MATCH_MP_TAC (last (CONJUNCTS aeq_rules)) THEN
-    SRW_TAC [][] THEN
-    METIS_TAC [rawpms_differing_types_commute]
-  ]);
+  Cases_on `ty = ty'`
+  >- (rw[] >> irule aeq_lam >>
+      qexists ‘lswapstr pi z’ >> rw[pmact_sing_to_back]) >>
+  rw[] >> irule aeq_lam >> rw[] >>
+  metis_tac [rawpms_differing_types_commute]
+QED
 
-val aeq_rawpml = store_thm(
-  "aeq_rawpml",
-  ``aeq (rawpm ty pi t1) t2 = aeq t1 (rawpm ty (REVERSE pi) t2)``,
-  METIS_TAC [rawpm_inverse, aeq_rawpm]);
+Theorem aeq_rawpml:
+  aeq (rhpm ty pi t1) t2 = aeq t1 (rhpm ty (REVERSE pi) t2)
+Proof
+  METIS_TAC [pmact_inverse, aeq_rawpm]
+QED
 
-val aeq_refl = Store_thm(
-  "aeq_refl",
-  ``aeq t t``,
+Theorem aeq_refl[simp]:
+  aeq t t
+Proof
   Induct_on `t` THEN SRW_TAC [][aeq_rules] THEN
   Cases_on `p` THEN
   Q_TAC (NEW_TAC "z") `q INSERT allvars r t` THEN
-  MATCH_MP_TAC (last (CONJUNCTS aeq_rules)) THEN
-  Q.EXISTS_TAC `z` THEN SRW_TAC [][aeq_rawpm]);
+  MATCH_MP_TAC aeq_lam THEN
+  Q.EXISTS_TAC `z` THEN SRW_TAC [][aeq_rawpm]
+QED
 
 val aeq_sym = store_thm(
   "aeq_sym",
@@ -173,19 +159,18 @@ val aeq_sym = store_thm(
   HO_MATCH_MP_TAC aeq_ind THEN SRW_TAC [][aeq_rules] THEN
   METIS_TAC [aeq_rules]);
 
-val aeq_app = store_thm(
-  "aeq_app",
+val aeq_app_rwt = store_thm(
+  "aeq_app_rwt",
   ``aeq (rhapp t u) z = ?z1 z2. (z = rhapp z1 z2) /\
                                 aeq t z1 /\ aeq u z2``,
   CONV_TAC (LAND_CONV (ONCE_REWRITE_CONV [aeq_cases])) THEN
   SRW_TAC [][]);
 
-val aeq_trans = store_thm(
-  "aeq_trans",
-  ``!s t u. aeq s t /\ aeq t u ==> aeq s u``,
-  Q_TAC SUFF_TAC `!s t. aeq s t ==> !u. aeq t u ==> aeq s u`
-        THEN1 METIS_TAC [] THEN
-  HO_MATCH_MP_TAC aeq_ind THEN SRW_TAC [][aeq_rules, aeq_app] THEN
+Theorem aeq_trans:
+  !s t u. aeq s t /\ aeq t u ==> aeq s u
+Proof
+  Induct_on ‘aeq’ >>
+  rw[aeq_rules, aeq_app_rwt] >>
   POP_ASSUM MP_TAC THEN
   CONV_TAC (LAND_CONV (ONCE_REWRITE_CONV [aeq_cases])) THEN
   SIMP_TAC (srw_ss()) [] THEN
@@ -195,58 +180,57 @@ val aeq_trans = store_thm(
   SRW_TAC [][] THEN
   Q_TAC (NEW_TAC "d") `{v;v1;v2;z;z'} UNION allvars ty t UNION
                        allvars ty u UNION allvars ty s` THEN
-  `!u'. aeq (rawpm ty [(d,z)] (rawpm ty [(z,v2)] u))
-            (rawpm ty [(d,z)] u') ==>
-        aeq (rawpm ty [(d,z)] (rawpm ty [(z,v1)] t))
-            (rawpm ty [(d,z)] u')`
+  ‘!u'. aeq (rhpm ty [(d,z)] (rhpm ty [(z,v2)] u))
+            (rhpm ty [(d,z)] u') ==>
+        aeq (rhpm ty [(d,z)] (rhpm ty [(z,v1)] t))
+            (rhpm ty [(d,z)] u')’
       by SRW_TAC [][aeq_rawpml] THEN
-  POP_ASSUM (Q.SPEC_THEN `rawpm ty [(d,z)] u'`
+  POP_ASSUM (Q.SPEC_THEN `rhpm ty [(d,z)] u'`
              (ASSUME_TAC o Q.GEN `u'` o
               SIMP_RULE (srw_ss()) [])) THEN
   POP_ASSUM (MP_TAC o
-             ONCE_REWRITE_RULE [GSYM rawpm_sing_to_back]) THEN
+             ONCE_REWRITE_RULE [GSYM pmact_sing_to_back]) THEN
   SRW_TAC [][allvars_fresh] THEN
-  `aeq (rawpm ty [(d,z')] (rawpm ty [(z',v2)] u))
-       (rawpm ty [(d,z')] (rawpm ty [(z',v)] s))`
+  ‘aeq (rhpm ty [(d,z')] (rhpm ty [(z',v2)] u))
+       (rhpm ty [(d,z')] (rhpm ty [(z',v)] s))’
      by SRW_TAC [][Once aeq_rawpml] THEN
-  POP_ASSUM (MP_TAC o ONCE_REWRITE_RULE [GSYM rawpm_sing_to_back]) THEN
-  SRW_TAC [][allvars_fresh, swapstr_def] THEN
-  METIS_TAC [aeq_rules]);
+  POP_ASSUM (MP_TAC o ONCE_REWRITE_RULE [GSYM pmact_sing_to_back]) THEN
+  SRW_TAC [][allvars_fresh] THEN
+  METIS_TAC [aeq_rules]
+QED
 
-val fv_def = Define`
+Definition fv_def[simp]:
   (fv ty (rhvar nty) = if ty = SND nty then {FST nty} else {}) /\
   (fv ty (rhconst nty) = {}) /\
   (fv ty (rhapp t1 t2) = fv ty t1 UNION fv ty t2) /\
   (fv ty (rhabs nty t) =
        if ty = SND nty then fv ty t DELETE FST nty
        else fv ty t)
-`;
-val _ = export_rewrites ["fv_def"]
+End
 
-val fv_SUBSET_allvars = store_thm(
-  "fv_SUBSET_allvars",
-  ``!x. x IN fv ty t ==> x IN allvars ty t``,
-  Induct_on `t` THEN SRW_TAC [][] THEN SRW_TAC [][]);
+Theorem fv_SUBSET_allvars:
+  !x. x IN fv ty t ==> x IN allvars ty t
+Proof
+  Induct_on `t` THEN SRW_TAC [][] THEN SRW_TAC [][]
+QED
 
 val IN_fv_rawpm = store_thm(
   "IN_fv_rawpm",
-  ``x IN fv ty (rawpm ty pi t) = lswapstr (REVERSE pi) x IN fv ty t``,
-  Induct_on `t` THEN SRW_TAC [][lswapstr_eql] THEN
+  ``x IN fv ty (rhpm ty pi t) ⇔ lswapstr (REVERSE pi) x IN fv ty t``,
+  Induct_on `t` THEN SRW_TAC [][pmact_eql] THEN
   FULL_SIMP_TAC (srw_ss()) []);
 
 val fv_rawpm_diff = store_thm(
   "fv_rawpm_diff",
-  ``~(ty = ty') ==> (fv ty (rawpm ty' pi t) = fv ty t)``,
+  ``~(ty = ty') ==> (fv ty (rhpm ty' pi t) = fv ty t)``,
   Induct_on `t` THEN SRW_TAC [][] THEN METIS_TAC []);
 
-
-val aeq_fv = store_thm(
-  "aeq_fv",
-  ``!t u. aeq t u ==> !ty. fv ty t = fv ty u``,
+Theorem aeq_fv:
+  !t u. aeq t u ==> !ty. fv ty t = fv ty u
+Proof
   HO_MATCH_MP_TAC aeq_ind THEN SRW_TAC [][EXTENSION] THEN
   COND_CASES_TAC THENL [
     SRW_TAC [][] THEN
-    SRW_TAC [][EXTENSION] THEN
     POP_ASSUM (Q.SPEC_THEN `ty` MP_TAC) THEN
     Cases_on `x = v1` THENL [
       SRW_TAC [][] THEN
@@ -265,29 +249,32 @@ val aeq_fv = store_thm(
     ],
     SRW_TAC [][] THEN FIRST_X_ASSUM (Q.SPEC_THEN `ty'` MP_TAC) THEN
     SRW_TAC [][fv_rawpm_diff]
-  ]);
+  ]
+QED
 
-val rhabs_respects_aeq = store_thm(
-  "rhabs_respects_aeq",
-  ``!t u. aeq t u ==> aeq (rhabs v t) (rhabs v u)``,
+Theorem rhabs_respects_aeq:
+  !t u. aeq t u ==> aeq (rhabs v t) (rhabs v u)
+Proof
   SRW_TAC [][] THEN Cases_on `v` THEN
   MATCH_MP_TAC (last (CONJUNCTS aeq_rules)) THEN
   Q_TAC (NEW_TAC "z") `q INSERT allvars r t UNION allvars r u` THEN
-  SRW_TAC [][aeq_rawpml] THEN METIS_TAC []);
+  SRW_TAC [][aeq_rawpml] THEN METIS_TAC []
+QED
 
-val alt_aeq_lam = store_thm(
-  "alt_aeq_lam",
-  ``(!z. ~(z IN allvars ty t1) /\ ~(z IN allvars ty t2) /\ ~(z = u) /\
-         ~(z = v) ==>
-         aeq (rawpm ty [(u,z)] t1) (rawpm ty [(v,z)] t2)) ==>
-    aeq (rhabs (u,ty) t1) (rhabs (v,ty) t2)``,
+Theorem alt_aeq_lam:
+  (!z. ~(z IN allvars ty t1) /\ ~(z IN allvars ty t2) /\ ~(z = u) /\
+       ~(z = v) ==>
+       aeq (rhpm ty [(u,z)] t1) (rhpm ty [(v,z)] t2)) ==>
+  aeq (rhabs (u,ty) t1) (rhabs (v,ty) t2)
+Proof
   STRIP_TAC THEN MATCH_MP_TAC (last (CONJUNCTS aeq_rules)) THEN
   Q_TAC (NEW_TAC "z") `allvars ty t1 UNION allvars ty t2 UNION {u;v}` THEN
-  METIS_TAC [rawpm_is_perm, is_perm_flip_args]);
+  METIS_TAC [rawpm_is_perm, pmact_flip_args]
+QED
 
-val fresh_swap = store_thm(
-  "fresh_swap",
-  ``!x y. ~(x IN fv ty t) /\ ~(y IN fv ty t) ==> aeq t (rawpm ty [(x,y)] t)``,
+Theorem fresh_swap:
+  !x y. x ∉ fv ty t ∧ y ∉ fv ty t ⇒ aeq t (rhpm ty [(x,y)] t)
+Proof
   Induct_on `t` THEN
   ASM_SIMP_TAC (srw_ss()) [aeq_rules, pairTheory.FORALL_PROD] THEN1
     SRW_TAC [][] THEN
@@ -299,30 +286,31 @@ val fresh_swap = store_thm(
     REPEAT STRIP_TAC THEN
     `~(z IN fv p_2 t)` by METIS_TAC [fv_SUBSET_allvars] THEN
     Cases_on `x = p_1` THEN ASM_SIMP_TAC (srw_ss()) [] THENL [
-      FULL_SIMP_TAC (srw_ss()) [is_perm_id] THEN
+      FULL_SIMP_TAC (srw_ss()) [pmact_id] THEN
       SRW_TAC [][] THEN
       Cases_on `y = p_1` THEN SRW_TAC [][] THEN
       CONV_TAC (RAND_CONV (RAND_CONV (ONCE_REWRITE_CONV
-                                        [GSYM rawpm_sing_to_back]))) THEN
+                                        [GSYM pmact_sing_to_back]))) THEN
       SRW_TAC [][],
       ALL_TAC
     ] THEN
     Cases_on `y = p_1` THEN SRW_TAC [][] THENL [
       FULL_SIMP_TAC (srw_ss()) [] THEN
       CONV_TAC (RAND_CONV (RAND_CONV (ONCE_REWRITE_CONV
-                                        [GSYM rawpm_sing_to_back]))) THEN
-      SRW_TAC [][is_perm_flip_args, rawpm_is_perm],
+                                        [GSYM pmact_sing_to_back]))) THEN
+      SRW_TAC [][pmact_flip_args],
       SRW_TAC [][]
     ],
     SRW_TAC [][rhabs_respects_aeq]
-  ]);
+  ]
+QED
 
-val aeq_lam_eqn = store_thm(
-  "aeq_lam_eqn",
-  ``(aeq (rhabs (n1,ty1) t1) (rhabs (n2,ty2) t2)) =
-      (ty1 = ty2) /\
-      ((n1 = n2) /\ aeq t1 t2 \/
-       ~(n1 = n2) /\ ~(n1 IN fv ty1 t2) /\ aeq t1 (rawpm ty1 [(n1,n2)] t2))``,
+Theorem aeq_lam_eqn:
+  aeq (rhabs (n1,ty1) t1) (rhabs (n2,ty2) t2) ⇔
+    ty1 = ty2 ∧
+    (n1 = n2 ∧ aeq t1 t2 \/
+     n1 ≠ n2 ∧ n1 ∉ fv ty1 t2 ∧ aeq t1 (rhpm ty1 [(n1,n2)] t2))
+Proof
   SIMP_TAC (srw_ss()) [EQ_IMP_THM, DISJ_IMP_THM] THEN REPEAT CONJ_TAC THENL [
     CONV_TAC (LAND_CONV (ONCE_REWRITE_CONV [aeq_cases])) THEN
     SRW_TAC [][] THEN
@@ -331,31 +319,31 @@ val aeq_lam_eqn = store_thm(
     Cases_on `n1 = n2` THEN1 FULL_SIMP_TAC (srw_ss()) [aeq_rawpml] THEN
     `~(n1 IN fv ty1 t2)`
        by (STRIP_TAC THEN
-           `n1 IN fv ty1 (rawpm ty1 [(z,n2)] t2)`
+           `n1 IN fv ty1 (rhpm ty1 [(z,n2)] t2)`
               by SRW_TAC [][IN_fv_rawpm] THEN
-           `n1 IN fv ty1 (rawpm ty1 [(z,n1)] t1)` by METIS_TAC [aeq_fv] THEN
+           `n1 IN fv ty1 (rhpm ty1 [(z,n1)] t1)` by METIS_TAC [aeq_fv] THEN
            FULL_SIMP_TAC (srw_ss()) [IN_fv_rawpm]) THEN
     FULL_SIMP_TAC (srw_ss()) [aeq_rawpml] THEN
-    Q.PAT_ASSUM `aeq X Y` MP_TAC THEN
-    ONCE_REWRITE_TAC [GSYM rawpm_sing_to_back] THEN
+    Q.PAT_X_ASSUM `aeq X Y` MP_TAC THEN
+    ONCE_REWRITE_TAC [GSYM pmact_sing_to_back] THEN
     SRW_TAC [][] THEN
     MATCH_MP_TAC aeq_trans THEN
-    Q.EXISTS_TAC `rawpm ty1 [(n1,n2)] (rawpm ty1 [(z,n1)] t2)` THEN
+    Q.EXISTS_TAC `rhpm ty1 [(n1,n2)] (rhpm ty1 [(z,n1)] t2)` THEN
     SRW_TAC [][] THEN
     SRW_TAC [][aeq_rawpml, fresh_swap],
 
     SRW_TAC [][] THENL [
       SRW_TAC [][rhabs_respects_aeq],
       MATCH_MP_TAC alt_aeq_lam THEN SRW_TAC [][aeq_rawpml] THEN
-      ONCE_REWRITE_TAC [GSYM rawpm_sing_to_back] THEN
+      ONCE_REWRITE_TAC [GSYM pmact_sing_to_back] THEN
       SRW_TAC [][] THEN
       `~(z IN fv ty1 t2)` by METIS_TAC [fv_SUBSET_allvars] THEN
       MATCH_MP_TAC aeq_trans THEN
-      Q.EXISTS_TAC `rawpm ty1 [(n1,n2)] t2` THEN SRW_TAC [][] THEN
-      SRW_TAC [][is_perm_flip_args, rawpm_is_perm, fresh_swap,
-                 aeq_rawpml]
+      Q.EXISTS_TAC `rhpm ty1 [(n1,n2)] t2` THEN SRW_TAC [][] THEN
+      SRW_TAC [][pmact_flip_args, fresh_swap, aeq_rawpml]
     ]
-  ]);
+  ]
+QED
 
 val aeq_equiv = prove(
   ``!t1 t2. aeq t1 t2 = (aeq t1 = aeq t2)``,
@@ -388,18 +376,20 @@ val aeq_fv' = prove(
                     (fv ty1 t1 = fv ty2 t2)``,
   SRW_TAC [][aeq_fv]);
 
-val aeq_rawpm' = prove(
+val aeq_rawpm0 = prove(
   ``!ty1 ty2 pi1 pi2 t u.
         (ty1 = ty2) /\ (pi1 = pi2) /\ aeq t u ==>
-        aeq (rawpm ty1 pi1 t) (rawpm ty2 pi2 u)``,
+        aeq (rhpm ty1 pi1 t) (rhpm ty2 pi2 u)``,
   SRW_TAC [][aeq_rawpm]);
 
-val [FV_thm, simple_induction, FINITE_FV, tpm_thm] =
+val aeq_rawpm' = SRULE [GSYM rawpm_rhpm] aeq_rawpm0
+
+val [FV_thm, simple_induction, FINITE_FV, raw_tpm_thm(*, tpm_is_pmact*)] =
     quotient.define_quotient_types_full {
       types = [{name = "term", equiv = aeq_equiv}],
       defs = map mk_def [("LAM", ``rhabs``), ("COMB", ``rhapp``),
                          ("VAR", ``rhvar``), ("CONST", ``rhconst``),
-                         ("FV", ``fv``), ("tpm", ``rawpm``)],
+                         ("FV", ``fv``), ("raw_tpm", ``rawpm``)],
       tyop_equivs = [],
       tyop_quotients = [],
       tyop_simps = [],
@@ -408,29 +398,27 @@ val [FV_thm, simple_induction, FINITE_FV, tpm_thm] =
       respects = [rhabs_respects, List.nth(CONJUNCTS aeq_rules, 2),
                   aeq_fv', aeq_rawpm', var_respects, con_respects],
       old_thms = [fv_def, TypeBase.induction_of ``:raw_holterm``,
-                  finite_fv, rawpm_def]
+                  finite_fv, rawpm_def(*, rawpm_is_perm*)]
 }
 
-val FV_thm = save_thm("FV_thm", FV_thm)
-val _ = export_rewrites ["FV_thm"]
-val simple_induction = save_thm("simple_induction", simple_induction)
-val FINITE_FV = save_thm("FINITE_FV", FINITE_FV)
-val _ = export_rewrites ["FINITE_FV"]
-val tpm_thm = save_thm("tpm_thm", tpm_thm)
-val _ = export_rewrites ["tpm_thm"]
+Theorem FV_thm[simp] = FV_thm
+Theorem simple_induction = simple_induction
+Theorem FINITE_FV[simp] = FINITE_FV
+Theorem raw_tpm_thm[simp] = raw_tpm_thm
 
-val tpm_is_perm = Store_thm(
-  "tpm_is_perm",
-  ``is_perm (tpm ty)``,
-  SRW_TAC [][is_perm_def] THENL [
+Theorem tpm_is_perm:
+  is_pmact (raw_tpm ty)
+Proof
+  SRW_TAC [][is_pmact_def] THENL [
     Q.ID_SPEC_TAC `x` THEN HO_MATCH_MP_TAC simple_induction THEN
     SRW_TAC [][],
     Q.ID_SPEC_TAC `x` THEN HO_MATCH_MP_TAC simple_induction THEN
-    SRW_TAC [][lswapstr_APPEND] THEN SRW_TAC [][] THEN
-    FULL_SIMP_TAC (srw_ss()) [],
-    FULL_SIMP_TAC (srw_ss()) [FUN_EQ_THM, permeq_def] THEN
-    HO_MATCH_MP_TAC simple_induction THEN SRW_TAC [][]
-  ]);
+    SRW_TAC [][pmact_decompose] THEN SRW_TAC [][] THEN
+    gs[],
+    simp[FUN_EQ_THM] >> Induct using simple_induction >>
+    SRW_TAC [][] >> metis_tac[pmact_permeq]
+  ]
+QED
 
 val _ = export_theory()
 
